Big changes (syntax/semantics) for easy reduction proof

src/Prototype/Language.v
@@ -7,26 +7,33 @@ Open Scope list.
 
 Section Language.
 
+  Definition IdxT := nat.
+
   (* A message is always either a request or a response.
    * A request indicates a start of a transaction.
    * A corresponding response indicates the end of the transaction.
    *)
-  Variable Msg: Type.
-  Variables (msg_is_req: Msg -> bool).
+  Variable MsgT: Type.
+  Inductive MsgType := Req | Resp.
+  Record Msg := { msg_type : MsgType;
+                  msg_from : IdxT;
+                  msg_to : IdxT;
+                  msg_content : MsgT }.
+  Definition buildMsg ty fr to co := {| msg_type := ty;
+                                        msg_from := fr;
+                                        msg_to := to;
+                                        msg_content := co |}.
   
   Section Syntax.
-
-    Definition IdxT := nat.
-    Definition IMsg := (IdxT * Msg)%type.
 
     Section Object.
       Variable StateT: Type.
 
       Definition CmdT :=
-        StateT -> option (list IMsg (* internal messages out *) *
-                          option IMsg (* optional external out *) *
+        StateT -> option (list Msg (* internal messages out *) *
+                          list Msg (* optional external out; the youngest should be the head *) *
                           StateT (* next state *)).
-      Definition RuleT := IMsg -> CmdT.
+      Definition RuleT := Msg -> CmdT.
 
       Record Object :=
         { obj_idx: nat;
@@ -50,24 +57,28 @@ Section Language.
     Definition ObjectStates :=
       Map IdxT { StateT : Type & ObjectState StateT }.
 
-    Definition InMsgs := Map IdxT (* from *) (list Msg).
+    Definition MsgsFrom := Map (IdxT * MsgType) (* (from, msgType) *) (list Msg).
+    Definition Messages := Map IdxT (* to *) MsgsFrom.
 
-    Definition ObjectInMsgs := Map (IdxT * bool) (* (to, is_req) *) InMsgs.
-
-    Definition idx_add {A} (k: IdxT) (v: A) m :=
-      add eq_nat_dec k v m.
-
-    Definition idx_bool_dec: forall (k1 k2: IdxT * bool), {k1 = k2} + {k1 <> k2}.
+    Definition idx_add {A} (k: IdxT) (v: A) m := add eq_nat_dec k v m.
+    Definition idx_msgType_dec: forall (k1 k2: IdxT * MsgType), {k1 = k2} + {k1 <> k2}.
     Proof.
       decide equality.
-      - apply Bool.bool_dec.
+      - decide equality.
       - apply eq_nat_dec.
     Defined.
-    Definition idx_bool_add {A} (k: IdxT * bool) (v: A) m :=
-      add idx_bool_dec k v m.
+    Definition idx_msgType_add {A} (k: IdxT * MsgType) (v: A) m :=
+      add idx_msgType_dec k v m.
+    Definition idx_idx_dec: forall (k1 k2: IdxT * IdxT), {k1 = k2} + {k1 <> k2}.
+    Proof.
+      decide equality; apply eq_nat_dec.
+    Defined.
+    Definition idx_idx_add {A} (k: IdxT * IdxT) (v: A) m :=
+      add idx_idx_dec k v m.
 
+    (* Return the result handled meaningfully first by a rule. *)
     Fixpoint step_rule {StateT} (rules: list (RuleT StateT))
-             (imsg: IMsg) (st: StateT) :=
+             (imsg: Msg) (st: StateT) :=
       match rules with
       | nil => None
       | r :: rules' =>
@@ -78,74 +89,74 @@ Section Language.
       end.
 
     Inductive step_obj {StateT}:
-      ObjectState StateT -> InMsgs ->
-      list IMsg -> option IMsg (* external_in *) -> option IMsg (* external_out *) ->
-      ObjectState StateT -> InMsgs -> Prop :=
-    | StepObjInt: forall os imsgs fidx fmsg fmsgs imsgs_to emsgs_to pos,
-        step_rule (obj_rules (os_obj os)) (fidx, fmsg) (os_state os) =
+      ObjectState StateT -> MsgsFrom ->
+      list Msg -> option Msg (* (possibly) external_in *) -> list Msg (* external_out *) ->
+      ObjectState StateT -> MsgsFrom -> Prop :=
+    | StepObjInt: forall os msgs_from fidx fmsgT fmsg fmsgs imsgs_to emsgs_to pos,
+        step_rule (obj_rules (os_obj os)) fmsg (os_state os) =
         Some (imsgs_to, emsgs_to, pos) ->
-        find fidx imsgs = Some (fmsg :: fmsgs) ->
-        step_obj os imsgs
+        find (fidx, fmsgT) msgs_from = Some (fmsg :: fmsgs) ->
+        step_obj os msgs_from
                  imsgs_to None emsgs_to
                  {| os_obj := os_obj os;
                     os_state := pos |}
-                 (idx_add fidx fmsgs imsgs)
-    | StepObjExt: forall os imsgs emsg_in imsgs_to emsgs_to pos,
+                 (idx_msgType_add (fidx, fmsgT) fmsgs msgs_from)
+    | StepObjExt: forall os msgs_from emsg_in imsgs_to emsgs_to pos,
         step_rule (obj_rules (os_obj os)) emsg_in (os_state os) =
         Some (imsgs_to, emsgs_to, pos) ->
-        step_obj os imsgs
+        step_obj os msgs_from
                  imsgs_to (Some emsg_in) emsgs_to
                  {| os_obj := os_obj os;
                     os_state := pos |}
-                 imsgs.
+                 msgs_from.
 
-    Fixpoint distr_msgs (from: IdxT) (to: list IMsg)
-             (msgs: ObjectInMsgs): ObjectInMsgs :=
+    Fixpoint distr_msgs (from: IdxT) (to: list Msg)
+             (msgs: Messages): Messages :=
       match to with
       | nil => msgs
-      | (toIdx, msg) :: to' =>
-        match find (toIdx, msg_is_req msg) msgs with
+      | msg :: to' =>
+        match find (msg_to msg) msgs with
         | Some toMsgs =>
-          let added := match toMsgs from with
+          let added := match toMsgs (from, msg_type msg) with
                        | Some fromMsgs => fromMsgs ++ (msg :: nil)
                        | None => msg :: nil
                        end in
-          idx_bool_add (toIdx, msg_is_req msg) (idx_add from added toMsgs) msgs
+          idx_add (msg_to msg) (idx_msgType_add (from, msg_type msg) added toMsgs) msgs
         | None =>
-          idx_bool_add (toIdx, msg_is_req msg) (idx_add from (msg :: nil) (@empty _ _)) msgs
+          idx_add (msg_to msg) (idx_msgType_add (from, msg_type msg) (msg :: nil) (@empty _ _)) msgs
         end
       end.
 
-    Inductive step : ObjectStates -> ObjectInMsgs ->
-                     option IMsg (* external in *) -> option IMsg (* external out *) ->
-                     ObjectStates -> ObjectInMsgs -> Prop :=
-    | Step: forall oss idx is_req {StateT} (os: ObjectState StateT)
-                   oims imsgs imsgs_to emsg_in emsg_out pos pimsgs,
+    Inductive step : ObjectStates -> Messages ->
+                     option Msg (* external in *) -> list Msg (* external out *) ->
+                     ObjectStates -> Messages -> Prop :=
+    | Step: forall oss idx {StateT} (os: ObjectState StateT)
+                   oims msgs_from imsgs_to emsg_in emsg_out pos pmsgs_from,
         find idx oss = Some (existT _ _ os) ->
-        find (idx, is_req) oims = Some imsgs -> 
-        step_obj os imsgs imsgs_to emsg_in emsg_out pos pimsgs ->
+        find idx oims = Some msgs_from -> 
+        step_obj os msgs_from imsgs_to emsg_in emsg_out pos pmsgs_from ->
         step oss oims emsg_in emsg_out
              (idx_add idx (existT _ _ pos) oss)
-             (distr_msgs idx imsgs_to (idx_bool_add (idx, is_req) pimsgs oims)).
+             (distr_msgs idx imsgs_to (idx_add idx pmsgs_from oims)).
 
     (* NOTE: the oldest is the head *)
-    Definition addHistory (om: option IMsg) (hst: list IMsg) :=
+    Definition addHistory (om: option Msg) (hst: list Msg) :=
       match om with
       | Some m => hst ++ (m :: nil)
       | None => hst
       end.
     Infix "<::" := addHistory (at level 30, right associativity).
 
-    Inductive steps : ObjectStates -> ObjectInMsgs ->
-                      list IMsg (* history *) ->
-                      ObjectStates -> ObjectInMsgs -> Prop :=
+    Inductive steps : ObjectStates -> Messages ->
+                      list Msg (* history *) ->
+                      ObjectStates -> Messages -> Prop :=
     | StepsNil: forall oss oims, steps oss oims nil oss oims
     | StepsCons:
         forall oss1 oims1 emsgs oss2 oims2,
           steps oss1 oims1 emsgs oss2 oims2 ->
           forall oss3 emsg_in emsg_out oims3,
             step oss2 oims2 emsg_in emsg_out oss3 oims3 ->
-            steps oss1 oims1 (emsg_out <:: emsg_in <:: emsgs) oss3 oims3.
+            steps oss1 oims1 (emsg_out ++ emsg_in <:: emsgs) oss3 oims3.
 
     Definition getObjectStateInit {StateT} (obj: Object StateT) :=
       {| os_obj := obj;
@@ -159,7 +170,7 @@ Section Language.
                 (getObjectStatesInit obs')
       end.
 
-    Definition HistoryOf (obs: Objects) (hst: list IMsg) :=
+    Definition HistoryOf (obs: Objects) (hst: list Msg) :=
       exists oss oims, steps (getObjectStatesInit obs) (@empty _ _) hst oss oims.
 
     (** Now some notions borrowed from linearlizability and serializability.
@@ -168,34 +179,58 @@ Section Language.
      *)
 
     (* A maximum subsequence of H consisting only of requests and matching responses. *)
-    Definition complete (hst: list IMsg): list IMsg. Admitted.
+    (* Should be a fancier implementation *)
+    Fixpoint complete' (hst: list Msg) : (list Msg * Map (IdxT (* request_from *) *
+                                                          IdxT (* request_to *)) nat) :=
+      match hst with
+      | nil => (nil, @empty _ _)
+      | msg :: hst' =>
+        let (chst, rs) := complete' hst' in
+        if msg_type msg then (* request *)
+          match find (msg_from msg, msg_to msg) rs with
+          | Some (S n) => (msg :: chst, idx_idx_add (msg_from msg, msg_to msg) n rs)
+          | _ => (chst, rs)
+          end
+        else (* response *)
+          (msg :: chst, idx_idx_add (msg_to msg, msg_from msg)
+                                    (match find (msg_to msg, msg_from msg) rs with
+                                     | Some n => S n
+                                     | None => 1
+                                     end) rs)
+      end.
 
-    Definition Complete (hst: list IMsg) := hst = complete hst.
+    Definition complete (hst: list Msg) := fst (complete' hst).
+    Definition Complete (hst: list Msg) := hst = complete hst.
 
-    Fixpoint Serial' (hst: list IMsg) (oi: option IdxT) :=
+    Fixpoint Serial' (hst: list Msg) (oi: option (IdxT (* request_from *) *
+                                                  IdxT (* request_to *))) :=
       match hst with
       | nil => True
-      | (idx, msg) :: hst' =>
+      | msg :: hst' =>
         match oi with
-        | Some i => idx = i /\ msg_is_req msg = false /\
-                    Serial' hst' None
-        | None => msg_is_req msg = true /\ Serial' hst' (Some idx)
+        | Some (from, to) => msg_to msg = from /\ msg_from msg = to /\ msg_type msg = Resp /\
+                             Serial' hst' None
+        | None => msg_type msg = Req /\ Serial' hst' (Some (msg_from msg, msg_to msg))
         end
       end.
 
-    Definition Serial (hst: list IMsg) := Serial' hst None.
+    Definition Serial (hst: list Msg) := Serial' hst None.
 
-    Definition subHistory (i: IdxT) (hst: list IMsg) :=
-      filter (fun e => if eq_nat_dec i (fst e) then true else false) hst.
+    Definition subHistory (i: IdxT) (hst: list Msg) :=
+      filter (fun e => if eq_nat_dec i (msg_to e) then true
+                       else if eq_nat_dec i (msg_from e) then true
+                            else false) hst.
 
-    Definition Equivalent (hst1 hst2: list IMsg) :=
+    Definition Equivalent (hst1 hst2: list Msg) :=
       forall i, subHistory i hst1 = subHistory i hst2.
 
-    Definition Serializable (hst: list IMsg) :=
-      exists shst, Serial shst /\ Equivalent (complete hst) shst.
+    Definition Serializable (hst shst: list Msg) :=
+      Serial shst /\ Equivalent (complete hst) shst.
 
     Definition SerialObjects (obs: Objects) :=
-      forall hst, HistoryOf obs hst -> Serializable hst.
+      forall hst,
+        HistoryOf obs hst ->
+        exists shst, HistoryOf obs shst /\ Serializable hst shst.
 
   End Semantics.
 
@@ -240,20 +275,21 @@ Section Language.
     Admitted.
     Hint Immediate complete_equivalent.
       
-    Lemma serial_serializable: forall hst, Serial hst -> Serializable hst.
+    Lemma serial_serializable: forall hst, Serial hst -> Serializable hst (complete hst).
     Proof.
-      intros; exists (complete hst); split; eauto.
+      intros; split; eauto.
     Qed.
     Hint Immediate serial_serializable.
 
     Lemma complete_serializable_app:
       forall hst1,
         Complete hst1 ->
-        forall hst2, Serializable hst2 -> Serializable (hst1 ++ hst2).
+        forall hst2 shst2, Serializable hst2 shst2 ->
+                           Serializable (hst1 ++ hst2) (hst1 ++ shst2).
     Proof.
       unfold Serializable; intros.
-      destruct H0 as [shst2 [? ?]].
-      exists (hst1 ++ shst2); split; auto.
+      destruct H0.
+      split; auto.
 
       rewrite complete_complete_app by assumption.
       apply equivalent_app; auto.
