src/Prototype/Correctness.v
@@ -1,7 +1,9 @@
 Require Import List String Peano_dec.
-Require Import Language SingleValue.
+Require Import FnMap Language SingleValue.
 
-Theorem impl_serial: SerialObjects svm_is_req impl.
+Theorem impl_serial: SerialObjects impl.
 Proof.
   unfold SerialObjects, HistoryOf, Serializable; intros.
+  destruct H as [oss [oims ?]].
+
 Admitted.
