src/Prototype/Reduction.v
@@ -1,0 +1,43 @@
+Require Import List String Peano_dec.
+Require Import FnMap Language.
+
+Section Reduction.
+  Variable MsgT: Type.
+  Definition Msg := Msg MsgT.
+
+  Definition Reduced (from to: list Msg) (msg1 msg2: Msg) :=
+    exists hst1 hst2,
+      from = hst1 ++ (msg1 :: msg2 :: hst2) /\
+      to = hst1 ++ (msg2 :: msg1 :: hst2).
+
+  Lemma reduction_preserved_steps':
+    forall msg1 msg2: Msg,
+      msg_from msg1 <> msg_from msg2 ->
+      forall oss1 oims1 oss2 oims2 hst2 hst1,
+        steps oss1 oims1 (hst1 ++ msg1 :: msg2 :: hst2) oss2 oims2 ->
+        steps oss1 oims1 (hst1 ++ msg2 :: msg1 :: hst2) oss2 oims2.
+  Proof.
+    induction hst1; simpl; intros.
+    - admit.
+    - admit.
+  Admitted.
+
+  Theorem reduction_preserved_steps:
+    forall oss1 oims1 hst oss2 oims2,
+      steps oss1 oims1 hst oss2 oims2 ->
+      forall msg1 msg2 hst',
+        Reduced hst hst' msg1 msg2 ->
+        msg_from msg1 <> msg_from msg2 -> (* Different sources -> 
+                                           * Messages were handled by different objects -> 
+                                           * Disjoint state transitions!
+                                           *)
+        steps oss1 oims1 hst' oss2 oims2.
+  Proof.
+    intros.
+    unfold Reduced; intros.
+    destruct H0 as [hst1 [hst2 [? ?]]]; subst.
+    apply reduction_preserved_steps'; auto.
+  Qed.
+
+End Reduction.
+        
